ElGamal/coq_src/powmod.v
@@ -1,29 +1,30 @@
 Require Import Hacspec_Lib MachineIntegers.
 From Coq Require Import ZArith.
 
-Definition uint128_pow_mod
-  (g_0: int128)
-  (x_1: int128)
-  (n_2: int128)
-
-  : int128 :=
-    (g_0 ^ x_1) mod n_2.
-  (**let asd_3 : int128 :=  **)
-  (** Z.powm(g_0 x_1 n_2). **)
-  
 Definition pow
   (g_3: int128)
   (x_4: int128)
   
   : int128 :=
-    g_3 ^ x_4.
+	repr (unsigned g_3 ^ unsigned x_4).
+    
     
 Definition uint128_modulo
 	(n_5: int128)
 	(n_6: int128)
 	
 	: int128 :=
-		n_5 mod n_6.
-    
+		MachineIntegers.modu n_5 n_6.
+
+Definition uint128_pow_mod
+  (g_0: int128)
+  (x_1: int128)
+  (n_2: int128)
+
+  : int128 :=
+    uint128_modulo (pow g_0 x_1) n_2.
+  (**let asd_3 : int128 :=  **)
+  (** Z.powm(g_0 x_1 n_2). **)
+  
     
 Notation "A .^^ B" := (pow A B) (at level 80). 
