Elgamal2/El_Gamal.v
@@ -1,0 +1,144 @@
+(** This file was automatically generated using Hacspec **)
+Set Warnings "-notation-overridden,-ambiguous-paths".
+From Crypt Require Import choice_type Package Prelude.
+Import PackageNotation.
+From extructures Require Import ord fset.
+From mathcomp.word Require Import ssrZ word.
+From Jasmin Require Import word.
+
+From Coq Require Import ZArith.
+Import List.ListNotations.
+Open Scope list_scope.
+Open Scope Z_scope.
+Open Scope bool_scope.
+
+
+From Hacspec Require Import ChoiceEquality.
+From Hacspec Require Import LocationUtility.
+From Hacspec Require Import Hacspec_Lib_Comparable.
+From Hacspec Require Import Hacspec_Lib_Pre.
+From Hacspec Require Import Hacspec_Lib.
+From Diffie Require Import powmod.
+
+Open Scope hacspec_scope.
+
+Obligation Tactic := try timeout 8 solve_ssprove_obligations.
+
+
+Definition q_v : int128 :=
+  @repr U128 29.
+
+Definition g_v : int128 :=
+  @repr U128 2.
+
+Definition secret_q_v : uint128 :=
+  secret (q_v).
+
+Definition secret_g_v : uint128 :=
+  secret (g_v).
+
+
+Notation "'enc_aux_inp'" :=(
+  uint128 '× int128 '× int128 : choice_type) (in custom pack_type at level 2).
+Notation "'enc_aux_inp'" :=(
+  uint128 '× int128 '× int128 : ChoiceEquality) (at level 2).
+Notation "'enc_aux_out'" :=((int128 '× int128
+  ) : choice_type) (in custom pack_type at level 2).
+Notation "'enc_aux_out'" :=((int128 '× int128) : ChoiceEquality) (at level 2).
+Definition ENC_AUX : nat :=
+  8.
+Program Definition enc_aux (secret_source_sk_4 : uint128) (
+    target_pk_0 : int128) (m_2 : int128)
+  : both (fset.fset0) [interface] ((int128 '× int128)) :=
+  ((letb secret_target_pk_1 : uint128 :=
+        uint128_classify (lift_to_both0 target_pk_0) in
+      letb secret_m_3 : uint128 := uint128_classify (lift_to_both0 m_2) in
+      letb secret_s_5 : uint128 :=
+        uint128_pow_mod (lift_to_both0 secret_target_pk_1) (
+          lift_to_both0 secret_source_sk_4) (lift_to_both0 secret_q_v) in
+      letb secret_c1_6 : uint128 :=
+        uint128_pow_mod (lift_to_both0 secret_g_v) (
+          lift_to_both0 secret_source_sk_4) (lift_to_both0 secret_q_v) in
+      letb secret_c2_7 : uint128 :=
+        uint128_modulo ((lift_to_both0 secret_m_3) .* (
+            lift_to_both0 secret_s_5)) (lift_to_both0 secret_q_v) in
+      lift_scope (H_loc_incl := _) (H_opsig_incl := _) (prod_b(
+          uint128_declassify (lift_to_both0 secret_c1_6),
+          uint128_declassify (lift_to_both0 secret_c2_7)
+        ))
+      ) : both (fset.fset0) [interface] ((int128 '× int128))).
+Fail Next Obligation.
+
+
+Notation "'keygen_inp'" :=(
+  unit_ChoiceEquality : choice_type) (in custom pack_type at level 2).
+Notation "'keygen_inp'" :=(unit_ChoiceEquality : ChoiceEquality) (at level 2).
+Notation "'keygen_out'" :=((int128 '× uint128
+  ) : choice_type) (in custom pack_type at level 2).
+Notation "'keygen_out'" :=((int128 '× uint128) : ChoiceEquality) (at level 2).
+Definition KEYGEN : nat :=
+  11.
+Program Definition keygen 
+  : both (fset.fset0) [interface] ((int128 '× uint128)) :=
+  ((letb secret_sk_9 : uint128 :=
+        uint128_classify (lift_to_both0 (@repr U128 4)) in
+      letb pk_10 : int128 :=
+        uint128_declassify (uint128_pow_mod (lift_to_both0 secret_g_v) (
+            lift_to_both0 secret_sk_9) (lift_to_both0 secret_q_v)) in
+      lift_scope (H_loc_incl := _) (H_opsig_incl := _) (prod_b(
+          lift_to_both0 pk_10,
+          lift_to_both0 secret_sk_9
+        ))
+      ) : both (fset.fset0) [interface] ((int128 '× uint128))).
+Fail Next Obligation.
+
+
+Notation "'enc_inp'" :=(
+  int128 '× int128 : choice_type) (in custom pack_type at level 2).
+Notation "'enc_inp'" :=(int128 '× int128 : ChoiceEquality) (at level 2).
+Notation "'enc_out'" :=((int128 '× int128
+  ) : choice_type) (in custom pack_type at level 2).
+Notation "'enc_out'" :=((int128 '× int128) : ChoiceEquality) (at level 2).
+Definition ENC : nat :=
+  16.
+Program Definition enc (target_pk_14 : int128) (m_15 : int128)
+  : both (fset.fset0) [interface] ((int128 '× int128)) :=
+  ((letb '(gy_12, y_13) : (int128 '× uint128) := keygen  in
+      lift_scope (H_loc_incl := _) (H_opsig_incl := _) (enc_aux (
+          lift_to_both0 y_13) (lift_to_both0 target_pk_14) (lift_to_both0 m_15))
+      ) : both (fset.fset0) [interface] ((int128 '× int128))).
+Fail Next Obligation.
+
+
+Notation "'dec_inp'" :=(uint128 '× (int128 '× int128
+  ) : choice_type) (in custom pack_type at level 2).
+Notation "'dec_inp'" :=(uint128 '× (int128 '× int128
+  ) : ChoiceEquality) (at level 2).
+Notation "'dec_out'" :=(int128 : choice_type) (in custom pack_type at level 2).
+Notation "'dec_out'" :=(int128 : ChoiceEquality) (at level 2).
+Definition DEC : nat :=
+  27.
+Program Definition dec (secret_target_sk_22 : uint128) (c_17 : (
+      int128 '×
+      int128
+    ))
+  : both (fset.fset0) [interface] (int128) :=
+  ((letb '(c1_18, c2_19) : (int128 '× int128) := lift_to_both0 c_17 in
+      letb secret_c1_20 : uint128 := uint128_classify (lift_to_both0 c1_18) in
+      letb secret_c2_21 : uint128 := uint128_classify (lift_to_both0 c2_19) in
+      letb secret_s_23 : uint128 :=
+        uint128_pow_mod (lift_to_both0 secret_c1_20) (
+          lift_to_both0 secret_target_sk_22) (lift_to_both0 secret_q_v) in
+      letb secret_s_inverse_24 : uint128 :=
+        uint128_pow_mod (lift_to_both0 secret_s_23) ((
+            lift_to_both0 secret_q_v) .- (lift_to_both0 secret_g_v)) (
+          lift_to_both0 secret_q_v) in
+      letb secret_m_25 : uint128 :=
+        uint128_pow_mod ((lift_to_both0 secret_c2_21) .* (
+            lift_to_both0 secret_s_inverse_24)) (uint128_classify (
+            lift_to_both0 (@repr U128 1))) (lift_to_both0 secret_q_v) in
+      letb m_26 : int128 := uint128_declassify (lift_to_both0 secret_m_25) in
+      lift_scope (H_loc_incl := _) (H_opsig_incl := _) (lift_to_both0 m_26)
+      ) : both (fset.fset0) [interface] (int128)).
+Fail Next Obligation.
+
