Elgamal2/nixfolder/pkgs.nix
@@ -1,0 +1,138 @@
+let
+  pkgs = import ./pin.nix { };
+  coqPackages = pkgs.coqPackages.overrideScope' (cfinal: cprev: {
+      coq = cprev.coq.override { version = "8.15.2"; };
+      mathcomp = cprev.mathcomp.override { 	version = "1.13.0"; };
+      mathcomp-analysis = cprev.mathcomp-analysis.override { version = "0.3.13"; };
+      mathcomp-word = cprev.mathcomp-word.override { version = "2.0"; };
+  });
+
+#	mathword = {
+#		owner = "jasmin-lang";
+#		repo = "coqword";
+#		rev = "960a955210b5fe08a610e868070ef61f35cb9a0b";
+#		sha256 = "Qu9tNgPC0nCu6C5HTR/S7AUGzuLFwErJ6q8M0St6w2Q=";
+#	};
+
+# coqword = coqPackages.callPackage ( { coq, stdenv, fetchFromGitHub, hierarchy-builder }:
+#    stdenv.mkDerivation {
+#      name = "coq${coq.coq-version}-coqword";
+
+#      src = fetchFromGitHub mathword;
+#      patchPhase = ''
+#          coq_makefile -f _CoqProject -o Makefile
+#      '';
+
+#      propagatedBuildInputs = [ coq pkgs.ocaml pkgs.dune_2 ] ++ (with coqPackages;
+#        [ deriving equations extructures mathcomp.ssreflect mathcomp-analysis mathcomp-word mathcomp-zify]);
+ #     enableParallelBuilding = true;
+ #     dontDetectOcamlConflicts = true;
+ #     installFlags = [ "COQLIB=$(out)/lib/coq/${coq.coq-version}/" ];
+ #   }
+ # ) { } ;
+  
+  jasmin-src = {
+    owner = "jasmin-lang";
+    repo = "jasmin";
+    rev = "3d40bc89a3426fd1b0c4f2fd6fb2767dbdf48554";
+    sha256 = "rnfC9wo7KAV0OFCIKkj1TullXDXcntn/8ewASFacPao=";
+  };
+  jasmin-proofs = coqPackages.callPackage ( { coq, stdenv, fetchFromGitHub }:
+    stdenv.mkDerivation {
+      name = "coq${coq.coq-version}-jasmin";
+      src = fetchFromGitHub jasmin-src + "/proofs";
+
+      propagatedBuildInputs = [ coq ] ++ (with coqPackages;
+        [ mathcomp.ssreflect mathcomp.algebra mathcomp-word ]);
+      enableParallelBuilding = true;
+      dontDetectOcamlConflicts = true;
+      installFlags = [ "COQLIB=$(out)/lib/coq/${coq.coq-version}/" ];
+    }
+  ) { } ;
+  ssprove = coqPackages.callPackage ( { coq, stdenv, fetchFromGitHub }:
+    stdenv.mkDerivation {
+      name = "coq${coq.coq-version}-ssprove";
+
+      src = fetchFromGitHub {
+        owner = "SSProve";
+        repo = "ssprove";
+        rev = "bead4e76acbb69b3ecf077cece56cd3fbde501e3";
+        sha256 = "sv69x3OqHilOXN9uzATsQxmzK8Z1k6V3ZZMq2dzbo1M=";
+      };
+      patchPhase = ''
+          coq_makefile -f _CoqProject -o Makefile
+      '';
+
+      propagatedBuildInputs = [ coq jasmin-proofs ] ++ (with coqPackages;
+        [ deriving equations extructures mathcomp.ssreflect mathcomp-analysis mathcomp-word mathcomp-zify ]);
+      enableParallelBuilding = true;
+      dontDetectOcamlConflicts = true;
+      installFlags = [ "COQLIB=$(out)/lib/coq/${coq.coq-version}/" ];
+    }
+  ) { } ;
+  hacspec-src = {
+    owner = "hacspec";
+    repo = "hacspec";
+    rev = "4ecc847fc944fe996e19423aa41f002f2039dab0";
+    sha256 = "65rPusiDe54DVO0ApLm/+vwAOc+mD5JOU7KUPJaJbSU=";
+  };
+
+  hacspec-coq = coqPackages.callPackage ( { coq, stdenv, fetchFromGitHub }:
+    stdenv.mkDerivation {
+      name = "coq${coq.coq-version}-hacspec-coq";
+      src = fetchFromGitHub hacspec-src + "/coq"; 
+
+        patchPhase = ''
+          coq_makefile -f _CoqProject -o Makefile
+   #       cat - >> ./src/Hacspec_Lib.v <<EOF
+    #      
+   #       Locate "^".
+ #         Definition uint128_pow_mod
+ #           (g_0: int128)
+  #          (x_1: int128)
+#            (n_2: int128)
+#
+ #           : int128 :=
+ #             (g_0 ^ x_1) mod n_2.
+  #        EOF
+ #         cat ./src/Hacspec_Lib.v
+        '';
+      
+
+      propagatedBuildInputs = with coqPackages; [ coq coqprime pkgs.ppl compcert QuickChick ];
+      enableParallelBuilding = true;
+      dontDetectOcamlConflicts = true;
+      installFlags = [ "COQLIB=$(out)/lib/coq/${coq.coq-version}/" ];
+    }
+  ) { } ;  
+  
+  hacspec-ssprove = coqPackages.callPackage ( { coq, stdenv, fetchFromGitHub }:
+    stdenv.mkDerivation {
+      name = "coq${coq.coq-version}-hacspec-ssprove";
+      src = fetchFromGitHub hacspec-src + "/coq_ssprove"; 
+
+      patchPhase = ''
+        coq_makefile -f _CoqProject -o Makefile
+ #       cat - >> ./src/Hacspec_Lib.v <<EOF
+ #       
+ #       Definition uint128_pow_mod
+ #         (g_0: int128)
+ #         (x_1: int128)
+ #         (n_2: int128)
+#
+ #         : int128 :=
+ #           (g_0 ^ x_1) mod n_2.
+ #       EOF
+ #       cat ./src/Hacspec_Lib.v
+      '';
+
+      propagatedBuildInputs = with coqPackages; [ coq ssprove mathcomp-word compcert pkgs.ppl ];
+      enableParallelBuilding = true;
+      dontDetectOcamlConflicts = true;
+      installFlags = [ "COQLIB=$(out)/lib/coq/${coq.coq-version}/" ];
+    }
+  ) { } ;
+  
+
+  coqide = coqPackages.coqide;
+in pkgs // { inherit ssprove hacspec-ssprove coqide hacspec-coq; }
